src/Curves/Edwards/XYZT/Readdition.v
@@ -39,6 +39,8 @@ Section ExtendedCoordinates.
   Local Notation coordinates := (coordinates(F:=F)(Feq:=Feq)(Fzero:=Fzero)(Fadd:=Fadd)(Fmul:=Fmul)(a:=a)(d:=d)).
   Context {a_eq_minus1:a = Fopp 1} {twice_d} {k_eq_2d:twice_d = d+d} {nonzero_d: d<>0}.
   Local Notation m1add := (m1add(F:=F)(Feq:=Feq)(Fzero:=Fzero)(Fone:=Fone)(Fopp:=Fopp)(Fadd:=Fadd)(Fsub:=Fsub)(Fmul:=Fmul)(Finv:=Finv)(Fdiv:=Fdiv)(field:=field)(char_ge_3:=char_ge_3)(Feq_dec:=Feq_dec)(a:=a)(d:=d)(nonzero_a:=nonzero_a)(square_a:=square_a)(nonsquare_d:=nonsquare_d)(a_eq_minus1:=a_eq_minus1)(twice_d:=twice_d)(k_eq_2d:=k_eq_2d)).
+  Local Notation zero := (zero(nonzero_a:=nonzero_a)).
+  Local Notation to_twisted := (to_twisted (nonzero_a:=nonzero_a)).
 
   (* Define a new cached point type *)
   Definition cached :=
@@ -65,23 +67,15 @@ Section ExtendedCoordinates.
     | _ => progress destruct_head' @Basic.point
     | _ => progress destruct_head' @cached
     | _ => progress destruct_head' and
-    | _ => progress cbv [eq CompleteEdwardsCurve.E.eq E.eq E.zero E.add E.opp fst snd cached_coordinates coordinates E.coordinates proj1_sig] in *
+    | _ => progress cbv [eq cached_eq CompleteEdwardsCurve.E.eq E.eq E.zero E.add E.opp fst snd cached_coordinates coordinates E.coordinates proj1_sig] in *
     | |- _ /\ _ => split | |- _ <-> _ => split
     end.
   Ltac t := repeat t_step; try Field.fsatz.
 
-  (* Stolen from Basic *)
-  Program Definition to_twisted (P:point) : Epoint :=
-    let XYZTT := coordinates P in let Ta := snd XYZTT in
-                                  let XYZT  := fst XYZTT in
-                                  let Tb := snd XYZT in
-                                  let XYZ := fst XYZT in      let Z := snd XYZ in
-                                                              let XY   := fst XYZ in       let Y := snd XY in
-                                                                                           let X    := fst XY in
-                                                                                           let iZ := Finv Z in ((X*iZ), (Y*iZ)).
-  Next Obligation. t. Qed.
-  Global Instance Proper_to_twisted : Proper (eq==>E.eq) to_twisted.
-  Proof using Type. cbv [to_twisted]; t. Qed.
+  Global Instance Equivalence_cached_eq : Equivalence cached_eq.
+  Proof using Feq_dec field nonzero_a twice_d nonzero_d k_eq_2d a_eq_minus1. split; repeat intro; t. Qed.
+  Global Instance DecidableRel_eq : Decidable.DecidableRel cached_eq.
+  Proof. intros P Q; destruct P as [ [ [ [ ] ? ] ? ] ?], Q as [ [ [ [ ] ? ] ? ] ? ]; exact _. Defined.
 
   Program Definition cached_to_twisted (C:cached) : Epoint :=
     let MPZT := cached_coordinates C in
@@ -94,6 +88,9 @@ Section ExtendedCoordinates.
             let iZ := Finv Z in (((hYpX-hYmX)*iZ), ((hYpX+hYmX)*iZ)).
   Next Obligation. t. Qed.
 
+  Global Instance Proper_cached_to_twisted : Proper (cached_eq==>E.eq) cached_to_twisted.
+  Proof using Type. cbv [cached_to_twisted]; t. Qed.
+
   Program Definition m1_prep (P : point) : cached :=
       match coordinates P return F*F*F*F with
         (X, Y, Z, Ta, Tb) =>
@@ -103,6 +100,11 @@ Section ExtendedCoordinates.
         (half_YmX, half_YpX, Z, Td)
       end.
   Next Obligation. t. Qed.
+
+  Global Instance Proper_m1_prep : Proper (eq==>cached_eq) m1_prep.
+  Proof using Type.
+    cbv [m1_prep]; t.
+  Qed.
 
   Program Definition m1_readd
       (P1 : point) (C : cached) : point :=
@@ -127,11 +129,144 @@ Section ExtendedCoordinates.
       => pose proof (E.denominator_nonzero _ nonzero_a square_a _ nonsquare_d _ _ (proj2_sig (to_twisted P1))  _ _  (proj2_sig (cached_to_twisted C)))
     end; t. Qed.
 
+  Global Instance Proper_m1_readd : Proper (eq==>cached_eq==>eq) m1_readd.
+  Proof using Type.
+    intros ? ? ? ? ? ?.
+    cbv [m1_readd]; t.
+  Qed.
+
   Create HintDb points_as_coordinates discriminated.
   Hint Unfold XYZT.Basic.point XYZT.Basic.coordinates XYZT.Basic.m1add
        E.point E.coordinates m1_readd m1_prep : points_as_coordinates.
   Lemma readd_correct P Q :
     Basic.eq (m1_readd P (m1_prep Q)) (m1add P Q).
   Proof. cbv [m1add m1_readd m1_prep]; t. Qed.
+
+(* TODO probably want this in a new scalar multiplication file, together with any other things I'll need for the proofs. *)
+Import PeanoNat.
+
+(* This exists already in a primer file for complete curves, but for E.point. Figure out which one I want to use.*)
+Fixpoint scalarmult (n : nat) (A : point) : point :=
+    match n with
+      | 0 => zero
+      | S n => m1add (scalarmult n A) A
+    end.
+
+  Lemma scalarmult_0 (A : point) : Logic.eq (scalarmult 0 A) zero.
+  Proof. cbv [scalarmult]; t; exact eq_refl. Qed.
+
+  (* TODO I don't *think* these are Logic.eq equal, just point equal. *)
+  Lemma scalarmult_1 (A : point) : Basic.eq (scalarmult 1 A) A.
+  Proof. cbv [scalarmult m1add zero]; t. Qed.
+  
+  Import Coq.Lists.List ListNotations. Local Open Scope list_scope.
+
+  (* Creates 0..(n-1)*A *)
+  Fixpoint multiples (n : nat) (A : point) : list point :=
+    match n with
+      | 0 => []
+      | S n => (multiples n A) ++ [(scalarmult n A)]
+    end.
+  
+  Lemma length_multiples (n : nat) (A : point) :
+    Logic.eq (List.length (multiples n A)) n.
+  Proof.
+    induction n.
+    - cbv [multiples length]. reflexivity.
+    - unfold multiples. fold multiples. rewrite length_app.
+      rewrite IHn. simpl. Lia.lia.
+  Qed.
+
+
+  Lemma multiples_correct (n : nat) (A : point) :
+    forall k default, k < n -> Logic.eq (List.nth k (multiples n A) default) (scalarmult k A).
+  Proof.
+    destruct n. intros. apply Nat.nlt_0_r in H. contradiction.
+    induction n.
+    - intros. assert (Logic.eq k 0%nat) by Lia.lia. subst. simpl. reflexivity.
+    - intros. unfold multiples. fold multiples. destruct (Nat.eq_dec k (S n)).
+      + subst. erewrite <- length_multiples at 1.
+        eapply nth_middle.
+      + erewrite app_nth1.
+        2: { rewrite length_app. erewrite length_multiples. simpl. Lia.lia. }
+        apply IHn. Lia.lia. 
+  Qed.
+
+  (* Nothing like this in stdlib, maybe I can add it? Or coqutil, if we have something there. *)
+  Lemma firstn_add {A} (n k : nat) (l : list A) : n <= length l -> Logic.eq (firstn (n + k) l) (firstn n l ++ firstn k (skipn n l)).
+  Proof.
+    intros.
+    replace l with (firstn n l ++ skipn n l) at 1. 2: { apply firstn_skipn. }
+    rewrite firstn_app. rewrite firstn_firstn. replace ((Init.Nat.min (n + k) n)) with n by Lia.lia.
+    rewrite length_firstn. replace (n + k - Init.Nat.min n (length l))%nat with k by Lia.lia.
+    reflexivity.
+  Qed.
+
+  Lemma firstn_pick_1 {A} (l : list A) default : forall n, n + 1 <= length l -> Logic.eq (firstn 1 (skipn n l)) ([nth n l default]).
+  Proof.
+    induction l.
+    - intros. inversion H. Lia.lia.
+    - intros. pose (IHl (n - 1)%nat). 
+        destruct n. simpl. reflexivity.
+        rewrite skipn_cons. replace (nth (S n) (a0 :: l) default) with (nth n l default) by auto.
+        replace (S n - 1)%nat with n in e by Lia.lia. apply e. simpl in H. Lia.lia.
+  Qed. 
+
+    Lemma firstn_pick_2 {A} (l : list A) default : forall n, n + 2 <= length l -> Logic.eq (firstn 2 (skipn n l)) ([nth n l default] ++ [nth (n + 1) l default]).
+  Proof.
+    intros.
+    replace 2%nat with (1 + 1)%nat by Lia.lia.
+    rewrite firstn_add. 2: { rewrite length_skipn. Lia.lia. }
+    rewrite (firstn_pick_1 _ default); [| Lia.lia].
+    rewrite skipn_skipn.
+    rewrite (firstn_pick_1 _ default); [| Lia.lia].
+    replace (1 + n)%nat with (n + 1)%nat by Lia.lia. reflexivity.
+  Qed.
+
+  (* didn't need those*)
+  Lemma multiples_app_index (n : nat) (A : point) :
+    forall i, i < n -> Logic.eq (multiples n A) ((firstn i (multiples n A)) ++ [scalarmult i A] ++ skipn (i + 1) (multiples n A)).
+  Proof.
+    intros.
+    eapply (nth_ext). Unshelve. 3,4: exact A.
+    - rewrite length_app, length_firstn, length_app, length_skipn, length_multiples. simpl. Lia.lia.
+    - rewrite length_multiples. 
+      intros. destruct (dec (n0 < i)).
+      + rewrite app_nth1. 2: { rewrite length_firstn, length_multiples. Lia.lia. }
+        rewrite nth_firstn. replace (n0 <? i) with true.
+        2:{ symmetry. rewrite Nat.ltb_lt. assumption. }
+        reflexivity.
+      + rewrite app_nth2. 2: { rewrite length_firstn, length_multiples. Lia.lia. } destruct (dec (n0 > i)).
+        * rewrite app_nth2. 2: {rewrite length_firstn, length_multiples. simpl. Lia.lia. }
+          rewrite nth_skipn, length_firstn, length_multiples. simpl.
+          replace ((i + 1 + (n0 - Init.Nat.min i n - 1))%nat) with n0.
+          2: {Lia.lia. } reflexivity.
+        * assert (Logic.eq i n0)%nat by Lia.lia.
+          rewrite app_nth1. 2: { rewrite length_firstn, length_multiples. simpl. Lia.lia. }
+          rewrite length_firstn, length_multiples. replace (n0 - Init.Nat.min i n)%nat with 0%nat.
+          rewrite multiples_correct. simpl. subst. reflexivity.
+          assumption. Lia.lia.
+  Qed. 
+
+  Lemma firstn_multiples (n : nat) (A : point) :
+    forall k, Logic.eq (firstn k (multiples n A)) (multiples (min k n) A).
+  Proof.
+    intros k.
+    eapply (nth_ext). Unshelve. 3,4: exact A.
+    - rewrite length_firstn, !length_multiples. Lia.lia.
+    - rewrite length_firstn, !length_multiples. intros ? ?. rewrite nth_firstn. 
+      rewrite !multiples_correct ; try Lia.lia.
+      replace (n0 <? k) with true.
+      2:{ symmetry. rewrite Nat.ltb_lt. Lia.lia. }
+      reflexivity.
+  Qed.
+
+  Lemma applast_multiples (n : nat) (A : point) :
+    n > 0 -> Logic.eq (multiples n A) ((multiples (n - 1) A) ++ [scalarmult (n - 1) A]).
+  Proof.
+    destruct n. intros. apply Nat.nlt_0_r in H. contradiction.
+    intros. replace (S n - 1)%nat with n by Lia.lia.
+    simpl. reflexivity.
+  Qed.  
 
 End ExtendedCoordinates.
