src/Bedrock/End2End/X25519/CachedMultiples.v
@@ -1,0 +1,588 @@
+Require Import bedrock2.Array.
+Require Import bedrock2.bottom_up_simpl.
+Require Import bedrock2.FE310CSemantics.
+Require Import bedrock2.Loops.
+Require Import bedrock2.Map.Separation.
+Require Import bedrock2.Map.SeparationLogic.
+Require Import bedrock2.NotationsCustomEntry.
+Require Import bedrock2.ProgramLogic.
+Require Import bedrock2.Scalars.
+Require Import bedrock2.Semantics.
+Require Import bedrock2.SepAutoArray.
+Require Import bedrock2.Syntax.
+Require Import bedrock2.WeakestPrecondition.
+Require Import bedrock2.WeakestPreconditionProperties.
+Require Import bedrock2.ZnWords.
+Require Import compiler.MMIO.
+Require Import compiler.Pipeline.
+Require Import compiler.Symbols.
+Require Import coqutil.Byte.
+Require Import coqutil.Map.Interface.
+Require Import coqutil.Map.OfListWord.
+From coqutil.Tactics Require Import Tactics letexists eabstract rdelta reference_to_string ident_of_string.
+Require Import coqutil.Word.Bitwidth32.
+Require Import coqutil.Word.Interface.
+Require Import coqutil.Word.Naive.
+From Coq Require Import Init.Byte.
+From Coq Require Import List.
+From Coq Require Import String.
+From Coq Require Import ZArith.
+Require Import Crypto.Arithmetic.PrimeFieldTheorems.
+Require Import Crypto.Bedrock.Field.Synthesis.New.UnsaturatedSolinas.
+Require Import Crypto.Bedrock.End2End.X25519.Field25519.
+Require Import Crypto.Bedrock.End2End.X25519.EdwardsXYZT. (* todo rename and move around properly, try to create a proper hierarchy of what needs what *)
+Require Import Crypto.Bedrock.Specs.Field.
+Require Import Crypto.Spec.Curve25519.
+Require Import Crypto.Util.Decidable.
+Require Import Crypto.Util.Tactics.DestructHead.
+Require Import Curves.Edwards.XYZT.Basic.
+Require Import Curves.Edwards.XYZT.Precomputed.
+Require Import Curves.Edwards.XYZT.Readdition.
+Require Import Lia.
+Require Crypto.Bedrock.Field.Synthesis.New.Signature.
+Local Open Scope string_scope.
+Local Open Scope Z_scope.
+Import LittleEndianList.
+Import ListNotations.
+Import ProgramLogic.Coercions.
+Import WeakestPrecondition.
+
+Local Existing Instance field_parameters.
+Local Existing Instance frep25519.
+Local Existing Instance frep25519_ok.
+
+(* Size of a field element in bytes. This is the same as computing eval in felem_size_bytes, but we want a notation instead of definition. *)
+Local Notation felem_size := 40.
+(* Size of a projective point in bytes. *)
+Local Notation pp_size := 200.
+(* Size of a cached point in bytes. *)
+Local Notation pc_size := 160.
+
+(* Notations help treat curve points like C structs. To avoid notation clashes, projective coordinates are capitalized. *)
+
+(* Member access notation for projective points: (X, Y, Z, Ta, Tb). *)
+Local Notation "A .X" := (A) (in custom bedrock_expr at level 2, left associativity, only parsing).
+Local Notation "A .Y" := (expr.op Syntax.bopname.add A (felem_size)) (in custom bedrock_expr at level 2, left associativity, only parsing).
+Local Notation "A .Z" := (expr.op Syntax.bopname.add A (felem_size + felem_size)) (in custom bedrock_expr at level 2, left associativity, only parsing).
+Local Notation "A .Ta" := (expr.op Syntax.bopname.add A (felem_size + felem_size + felem_size)) (in custom bedrock_expr at level 2, left associativity, only parsing).
+Local Notation "A .Tb" := (expr.op Syntax.bopname.add A (felem_size + felem_size + felem_size + felem_size)) (in custom bedrock_expr at level 2, left associativity, only parsing).
+
+(* Member access notation for cached points: (half_YmX, half_YpX, Z, Td). *)
+Local Notation "A .half_YmX" := (A) (in custom bedrock_expr at level 2, left associativity, only parsing).
+Local Notation "A .half_YpX" := (expr.op Syntax.bopname.add A (felem_size)) (in custom bedrock_expr at level 2, left associativity, only parsing).
+Local Notation "A .Z" := (expr.op Syntax.bopname.add A (felem_size + felem_size)) (in custom bedrock_expr at level 2, left associativity, only parsing).
+Local Notation "A .Td" := (expr.op Syntax.bopname.add A (felem_size + felem_size + felem_size)) (in custom bedrock_expr at level 2, left associativity, only parsing).
+
+(* Input is a projective point p, output is multiples of p as cached points, to be used for scalar multiplication. *)
+Definition cached_multiples := func! (p_ai, p_a, p_d) {
+  (* The first point is 0*A, so just zero. *)
+  stackalloc pp_size as zero;
+  zero_projective_point(zero);
+  to_cached(p_ai, zero, p_d);
+
+  (* The second point is 1*A.*)
+  to_cached(p_ai+$pc_size, p_a, p_d);
+
+  (* Helper array of normal points for double and add results, contains multiples of A, 1-7. *)
+  stackalloc 7*pp_size as p_ai_uncached;
+  (* copy 1*A into the helper array at index 0. *)
+  copy_projective_point(p_ai_uncached, p_a);
+
+  (* Remaining points are generated in a loop. *)
+  i = $2;
+  stackalloc pp_size as temp;
+  while (i < $16) {
+    double(temp, p_ai_uncached+(((i >> $1) - $1) * $pp_size)); (* Double (i/2)*A, now temp contains i*A. *)
+    to_cached(p_ai+(i*$pc_size), temp, p_d); (* copy temp to Ai *)
+    if (i < $8) {
+      (* Save i*A for later, at index i. *)
+      copy_projective_point(p_ai_uncached+((i - $1)*$pp_size), temp)
+    };
+    (* Now for the odd numbers, calculate (i+1)*A, store in temp. *)
+    readd(temp, p_a, p_ai+(i*$pc_size));
+    (* Store (i+1)*A in the result array. *)
+    to_cached(p_ai+((i+$1)*$pc_size), temp, p_d);
+    if (i < $7) {
+      (* Save (i+1)*A for later. *)
+      copy_projective_point(p_ai_uncached+(i*$pp_size), temp)
+    };
+    i = i + $2
+  }
+}.
+
+Section WithParameters.
+Context {two_lt_M: 2 < M_pos}.
+(* TODO: Can we provide actual values/proofs for these, rather than just sticking them in the context? *)
+Context {char_ge_3 : (@Ring.char_ge (F M_pos) Logic.eq F.zero F.one F.opp F.add F.sub F.mul (BinNat.N.succ_pos BinNat.N.two))}.
+Context {field:@Algebra.Hierarchy.field (F M_pos) Logic.eq F.zero F.one F.opp F.add F.sub F.mul F.inv F.div}.
+Context {a d: F M_pos}
+        {nonzero_a : a <> F.zero}
+        {square_a : exists sqrt_a, (F.mul sqrt_a sqrt_a) = a}
+        {nonsquare_d : forall x, (F.mul x x) <> d}.
+Context {a_eq_minus1:a = F.opp F.one} {twice_d} {k_eq_2d:twice_d = (F.add d d)} {nonzero_d: d<>F.zero}.
+
+(* Avoid unfolding deeper than necessary. *)
+(*Local Opaque F.to_Z word.rep word.wrap word.unsigned word.of_Z word.add feval.*)
+
+Local Notation "m =* P" := ((P%sep) m) (at level 70, only parsing).
+
+Local Notation zero := (zero(nonzero_a:=nonzero_a)).
+
+Local Notation FElem := (FElem(FieldRepresentation:=frep25519)).
+Local Notation felem_size_in_bytes := (felem_size_in_bytes(FieldRepresentation:=frep25519)).
+Local Notation bounded_by := (bounded_by(FieldRepresentation:=frep25519)).
+Local Notation word := (Naive.word 32).
+Local Notation felem := (felem(FieldRepresentation:=frep25519)).
+Local Notation point := (point(Feq:=Logic.eq)(Fzero:=F.zero)(Fadd:=F.add)(Fmul:=F.mul)(a:=a)(d:=d)).
+Local Notation cached := (cached(Fzero:=F.zero)(Fadd:=F.add)(Fmul:=F.mul)(a:=a)(d:=d)).
+Local Notation coordinates := (coordinates(Fzero:=F.zero)(Fadd:=F.add)(Fmul:=F.mul)(Feq:=Logic.eq)(a:=a)(d:=d)).
+Local Notation cached_coordinates := (cached_coordinates(Fzero:=F.zero)(Fadd:=F.add)(Fdiv:=F.div)(Fmul:=F.mul)(Fsub:=F.sub)(Feq:=Logic.eq)(a:=a)(d:=d)).
+Local Notation m1double :=
+  (m1double(F:=F M_pos)(Feq:=Logic.eq)(Fzero:=F.zero)(Fone:=F.one)
+           (Fopp:=F.opp)(Fadd:=F.add)(Fsub:=F.sub)(Fmul:=F.mul)(Finv:=F.inv)(Fdiv:=F.div)
+           (field:=field)(char_ge_3:=char_ge_3)(Feq_dec:=F.eq_dec)
+           (a:=a)(d:=d)(nonzero_a:=nonzero_a)(square_a:=square_a)(nonsquare_d:=nonsquare_d)
+           (a_eq_minus1:=a_eq_minus1)(twice_d:=twice_d)(k_eq_2d:=k_eq_2d)).
+Local Notation m1_readd :=
+  (m1_readd(F:=F M_pos)(Feq:=Logic.eq)(Fzero:=F.zero)(Fone:=F.one)
+           (Fopp:=F.opp)(Fadd:=F.add)(Fsub:=F.sub)(Fmul:=F.mul)(Finv:=F.inv)(Fdiv:=F.div)
+           (field:=field)(char_ge_3:=char_ge_3)(Feq_dec:=F.eq_dec)
+           (a:=a)(d:=d)(nonzero_a:=nonzero_a)(square_a:=square_a)(nonsquare_d:=nonsquare_d)
+           (a_eq_minus1:=a_eq_minus1)(twice_d:=twice_d)(k_eq_2d:=k_eq_2d)(nonzero_d:=nonzero_d)).
+Local Notation readd_correct :=
+  (readd_correct(F:=F M_pos)(Feq:=Logic.eq)(Fzero:=F.zero)(Fone:=F.one)
+                  (Fopp:=F.opp)(Fadd:=F.add)(Fsub:=F.sub)(Fmul:=F.mul)(Finv:=F.inv)(Fdiv:=F.div)
+                  (field:=field)(char_ge_3:=char_ge_3)(Feq_dec:=F.eq_dec)
+                  (a:=a)(d:=d)(nonzero_a:=nonzero_a)(a_eq_minus1:=a_eq_minus1)
+                  (twice_d:=twice_d)(k_eq_2d:=k_eq_2d)(square_a:=square_a)(nonsquare_d:=nonsquare_d)(nonzero_d:=nonzero_d)). 
+Local Notation m1_prep :=
+  (m1_prep(F:=F M_pos)(Feq:=Logic.eq)(Fzero:=F.zero)(Fone:=F.one)
+                  (Fopp:=F.opp)(Fadd:=F.add)(Fsub:=F.sub)(Fmul:=F.mul)(Finv:=F.inv)(Fdiv:=F.div)
+                  (field:=field)(char_ge_3:=char_ge_3)(Feq_dec:=F.eq_dec)
+                  (a:=a)(d:=d)(nonzero_a:=nonzero_a)(a_eq_minus1:=a_eq_minus1)
+                  (twice_d:=twice_d)(k_eq_2d:=k_eq_2d)(nonzero_d:=nonzero_d)). 
+Local Notation multiples :=
+  (multiples(F:=F M_pos)(Feq:=Logic.eq)(Fzero:=F.zero)(Fone:=F.one)
+                  (Fopp:=F.opp)(Fadd:=F.add)(Fsub:=F.sub)(Fmul:=F.mul)(Finv:=F.inv)(Fdiv:=F.div)
+                  (field:=field)(char_ge_3:=char_ge_3)(Feq_dec:=F.eq_dec)
+                  (a:=a)(d:=d)(nonzero_a:=nonzero_a)(a_eq_minus1:=a_eq_minus1)
+                  (twice_d:=twice_d)(k_eq_2d:=k_eq_2d)(square_a:=square_a)(nonsquare_d:=nonsquare_d)). 
+Local Notation scalarmult :=
+  (scalarmult(F:=F M_pos)(Feq:=Logic.eq)(Fzero:=F.zero)(Fone:=F.one)
+                  (Fopp:=F.opp)(Fadd:=F.add)(Fsub:=F.sub)(Fmul:=F.mul)(Finv:=F.inv)(Fdiv:=F.div)
+                  (field:=field)(char_ge_3:=char_ge_3)(Feq_dec:=F.eq_dec)
+                  (a:=a)(d:=d)(nonzero_a:=nonzero_a)(a_eq_minus1:=a_eq_minus1)
+                  (twice_d:=twice_d)(k_eq_2d:=k_eq_2d)(square_a:=square_a)(nonsquare_d:=nonsquare_d)). 
+Local Notation m1add := (m1add(F:=F M_pos)(Feq:=Logic.eq)(Fzero:=F.zero)(Fone:=F.one)
+           (Fopp:=F.opp)(Fadd:=F.add)(Fsub:=F.sub)(Fmul:=F.mul)(Finv:=F.inv)(Fdiv:=F.div)
+           (field:=field)(char_ge_3:=char_ge_3)(Feq_dec:=F.eq_dec)
+           (a:=a)(d:=d)(nonzero_a:=nonzero_a)(square_a:=square_a)(nonsquare_d:=nonsquare_d)
+           (a_eq_minus1:=a_eq_minus1) (twice_d:=twice_d) (k_eq_2d:=k_eq_2d)).
+
+Local Notation "p .+ n" := (word.add p (word.of_Z n)) (at level 50, format "p .+ n", left associativity).
+Local Notation "c 'p5@' p" := (p5at c p) (at level 10, format "c 'p5@' p").
+Local Notation "c 'p4@' p" := (p4at c p) (at level 10, format "c 'p4@' p").
+
+Definition cached_point (p : word) (a : cached) : map.rep -> Prop :=
+  Lift1Prop.ex1 (fun a_repr : cached_repr a => (a_repr p4@ p)).
+Definition projective_point (p : word) (a : point) : map.rep -> Prop :=
+  Lift1Prop.ex1 (fun a_repr : projective_repr a => (a_repr p5@ p)).
+
+From Coq Require Import Morphisms.
+
+Lemma projective_point_proper : Proper (Logic.eq==>Basic.eq==>Logic.eq==>Logic.eq) projective_point.
+Proof.
+  intros ? ? ? ? ? ? ? ? ?. subst.
+  cbv [projective_point].
+  (*assume this and check if this actually works.. I don't even know if this is true though*)
+Admitted.
+
+Instance spec_of_cached_multiples : spec_of "cached_multiples" :=
+  fnspec! "cached_multiples"
+    (p_ai p_a p_d: word) /
+    (a : point) (a_repr : projective_repr a) (d1: felem) (out : list byte) (R : _ -> Prop), {
+      requires t m :=
+        m =* out $@ p_ai * a_repr p5@ p_a * FElem p_d d1 *  R /\
+        Datatypes.length out = Z.to_nat (16*pc_size) /\
+        d = feval d1 /\
+        bounded_by tight_bounds d1;
+      ensures t' m' :=
+        t = t' /\
+        exists (mult_a : list cached), List.Forall2 (cached_eq) mult_a (List.map m1_prep (multiples 16 a)) /\
+        m' =* (array cached_point (word.of_Z pc_size) p_ai mult_a) * a_repr p5@ p_a * FElem p_d d1 * R
+    }.
+
+Local Ltac cbv_bounds H :=
+  cbv [un_xbounds bin_xbounds bin_ybounds un_square bin_mul bin_add bin_carry_add bin_sub bin_carry_sub un_outbounds bin_outbounds] in H;
+  cbv [un_xbounds bin_xbounds bin_ybounds un_square bin_mul bin_add bin_carry_add bin_sub bin_carry_sub un_outbounds bin_outbounds].
+
+Local Ltac solve_bounds :=
+  repeat match goal with
+  | H: bounded_by loose_bounds ?x |- bounded_by loose_bounds ?x => apply H
+  | H: bounded_by tight_bounds ?x |- bounded_by tight_bounds ?x => apply H
+  | H: bounded_by tight_bounds ?x |- bounded_by loose_bounds ?x => apply relax_bounds
+  | H: bounded_by _ ?x |- bounded_by _ ?x => cbv_bounds H
+  end.
+
+  Ltac solve_nums := 
+    repeat match goal with
+          | |- context [Datatypes.length (skipn _ _)] => rewrite !length_skipn
+          | |- context [Datatypes.length (multiples _ _)] => rewrite !length_multiples
+          | |- context [Datatypes.length (firstn _ _)] => rewrite !length_firstn
+        end; solve [lia|listZnWords].
+
+Ltac skipn_firstn_length :=
+  change felem_size_in_bytes with 40 in *; solve_nums.
+
+Ltac split_stack_at_n_in stack p n H := rewrite <- (firstn_skipn n stack) in H;
+  rewrite (map.of_list_word_at_app_n _ _ _ n) in H; try skipn_firstn_length;
+  let D := fresh in unshelve(epose (sep_eq_putmany _ _ (map.adjacent_arrays_disjoint_n p (firstn n stack) (skipn n stack) n _ _)) as D); [skipn_firstn_length|skipn_firstn_length|];
+  seprewrite_in D H; rewrite ?skipn_skipn in H; bottom_up_simpl_in_hyp H; clear D.
+
+Local Ltac solve_mem :=
+  try match goal with  | |- exists _ : _ -> Prop, _%sep _ => eexists end;
+  match goal with  | H : _ %sep ?m |- _ %sep ?m => bottom_up_simpl_in_goal_nop_ok end;
+  match goal with
+  | |- _%sep _ => ecancel_assumption_impl
+  | H: ?P%sep ?m |- ?G%sep ?m =>  (* Solve Placeholder goals when a fixed size list is given *)
+    match P with context[map.of_list_word_at ?p ?stack] =>
+    match G with context[Placeholder ?p _] =>
+      solve [ cbv [Placeholder]; extract_ex1_and_emp_in_goal; bottom_up_simpl_in_goal_nop_ok; split; [ecancel_assumption | skipn_firstn_length] ]
+    end end
+  end.
+
+Local Ltac single_step :=
+  repeat straightline; straightline_call; ssplit; try solve_mem; try solve_bounds;
+  (* solve simple preconditions *) try solve_nums; try assumption.
+
+(* p5@ -> $@, I want to match on p5@ but I don't know how *)
+Hint Extern 1 (Lift1Prop.impl1 (_) (sepclause_of_map (_ $@ ?p))) => (apply p5_impl_bytes) : ecancel_impl.
+
+Local Instance spec_of_zero_projective_point: spec_of "zero_projective_point" := spec_of_zero_projective_point (a:=a) (d:=d) (nonzero_a:=nonzero_a).
+Local Instance spec_of_to_cached : spec_of "to_cached" := spec_of_to_cached (nonzero_d:=nonzero_d) (k_eq_2d:=k_eq_2d) (twice_d:=twice_d) (a_eq_minus1:=a_eq_minus1) (nonzero_a:=nonzero_a) (d:=d) (a:=a).
+Local Instance spec_of_copy_projective_point : spec_of "copy_projective_point" := spec_of_copy_projective_point (a:=a) (d:=d).
+Local Instance spec_of_double : spec_of "double" := spec_of_double (k_eq_2d:=k_eq_2d) (a_eq_minus1:=a_eq_minus1) (nonsquare_d:=nonsquare_d) (square_a:=square_a) (nonzero_a:=nonzero_a) (a:=a) (d:=d) (twice_d:=twice_d).
+Local Instance spec_of_of_readd : spec_of "readd" := spec_of_readd (nonzero_d:=nonzero_d) (k_eq_2d:=k_eq_2d) (twice_d:=twice_d) (a_eq_minus1:=a_eq_minus1) (nonsquare_d:=nonsquare_d) (square_a:=square_a) (nonzero_a:=nonzero_a) (d:=d) (a:=a).
+
+(* TODO remove this later, I don't want it here.*)
+Local Ltac destruct_points :=
+  repeat match goal with
+    | _ => progress destruct_head' @Readdition.cached
+    | _ => progress destruct_head' cached_repr
+    | _ => progress destruct_head' @Basic.point
+    | _ => progress destruct_head' projective_repr
+    | _ => progress destruct_head' @precomputed_point
+    | _ => progress destruct_head' precomputed_repr
+    | _ => progress destruct_head' prod
+    | _ => progress destruct_head' and
+    | _ => progress lazy beta match zeta delta [p5at p4at coordinates precomputed_coordinates cached_coordinates proj1_sig] in *
+  end.
+
+Lemma cached_multiples_ok: program_logic_goal_for_function! cached_multiples.
+Proof.
+   (* Without this, resolution of cbv stalls out Qed. *)
+   (* TODO can't I mark these as opaque in this section and the locally, in a tactic unopaque them when needed. (Or opaque below, where the actual harm happens, which is probably modulo arithmetics.)*)
+  Strategy -1000 [un_xbounds bin_xbounds bin_ybounds un_square bin_mul bin_add bin_carry_add bin_sub bin_carry_sub un_outbounds bin_outbounds].
+
+
+  (* put zero into ai[0] *)
+  repeat straightline.
+  seprewrite_in array1_iff_eq_of_list_word_at H9; [solve_nums|].
+  single_step.
+  repeat straightline.
+  split_stack_at_n_in out p_ai 160%nat H21. (* split out ai[0] *)
+  single_step.
+  
+  (* put A into ai[1] *)
+  repeat straightline.
+  split_stack_at_n_in (skipn 160 out) (p_ai.+160) 160%nat H22. (* split out ai[1]*)
+  single_step.
+
+  (* allocate helper array (and split it up here already? might make stuff slow) *)
+  repeat straightline.
+  seprewrite_in array1_iff_eq_of_list_word_at H23; [solve_nums|]. (* because allocation uses array, best way is to build a switch for allocation to use $@. *)
+
+  (* copy over 1*A to p_ai_uncached *)
+  split_stack_at_n_in stack1 a4 200%nat H23. (* index 0, stores A*1*)
+  single_step.
+  repeat straightline. 
+
+  (* Loop! *)
+  refine (tailrec
+            (* I think R may change, so it'd be nice to have here, let's see.  *)
+            (HList.polymorphic_list.cons (_(*R'*))
+              (HList.polymorphic_list.cons (_(*temp_value*)) HList.polymorphic_list.nil))
+            (*variables*)(["temp"; "i"; "p_ai_uncached"; "zero"; "p_a"; "p_d"; "p_ai"]) (* these must be all variables we have, even if we don't use them*)
+            (*spec*)(fun v R' temp_value t m temp i p_ai_uncached zero p_a p_d p_ai=>
+                let i_z := word.unsigned i in
+                PrimitivePair.pair.mk
+                  (* Invariant *)
+                  (v = (8 - i_z / 2) /\
+                   i_z mod 2 = 0 /\ 2 <= i_z < 16 /\
+                   m =* 
+                        (* p_ai contains 0 - (i-1) of cached_multiples *)
+                        array cached_point (word.of_Z pc_size) p_ai (map m1_prep (multiples (Z.to_nat (i_z)) a0)) *
+                        (* the remaining space of p_ai is unused*)
+                        (skipn (Z.to_nat ((i_z) * pc_size)) out) $@ (p_ai .+ ((i_z) * pc_size)) *
+                        (* p_ai_uncached contains 1 - (i-1) of uncached_multiples, maximum 1-7 *)
+                        array projective_point (word.of_Z pp_size)
+                          (p_ai_uncached) (skipn 1 (multiples (Z.to_nat (i_z)) a0)) *
+                        (* and (if there is any), the rest of its memory is unused *)
+                        (skipn (Z.to_nat ((i_z - 1) * pp_size)) stack1) $@ (p_ai_uncached .+ ((i_z - 1) * pp_size)) *
+                        (* temp can be anything, it's only used within the loop *)
+                        temp_value $@ temp *
+                        (* remaining memory is left untouched *)
+                        a_repr p5@ p_a * FElem p_d d1 * R' /\
+                        Datatypes.length temp_value = Z.to_nat pp_size)
+                  (* Postcondition Schema *)
+                  (fun T_f M_f temp_f i_f p_ai_uncached_f zero_f p_a_f p_d_f p_ai_f =>
+                     T_f = t /\ 
+                     M_f =* array cached_point (word.of_Z pc_size) p_ai (map m1_prep (multiples 16 a0)) *
+                            array projective_point (word.of_Z pp_size)
+                          (p_ai_uncached) (skipn 1 (multiples (Z.to_nat (i_z)) a0)) *
+                            (* todo temp *)
+                            a_repr p5@ p_a * FElem p_d d1 * R')) (* TODO R' here? maybe R? not sure*)
+            (*measure*)(fun n m : Z => 0 <= n < m) _ _ _ _ _ _ _); loop_simpl.
+
+  { repeat straightline. }
+  { exact (Z.lt_wf _). }
+  {
+    repeat straightline.
+    ssplit. 1, 2, 3:solve_nums.
+    bottom_up_simpl_in_goal.
+
+    (* Doesn't seem to exist yet for nat? *)
+    Ltac isNatCst n := match n with 
+      | 0%nat => constr:(true)
+      | S ?k => isNatCst k
+      | _ => constr:(false)
+    end.
+
+    (* TODO expand this to a generic tactic that simplifies all the obvious list stuff. *)
+    Ltac simplify_lists_in_goal := 
+    repeat multimatch goal with
+      (* unfold constant subset of multiples *)
+      | |- context [multiples ?n ?a] => lazymatch isNatCst n with true =>
+        let v := eval cbv [multiples app] in (multiples n a) in change (multiples n a) with v
+      end
+      (* pull skipn into nth *)
+      | |- context [nth _ (skipn _ _)] => rewrite nth_skipn
+      (* resolve nth of multiples *)
+      | |- context [nth _ (multiples _ _)] => rewrite multiples_correct; [|solve_nums] (* todo rename to nth multiples*)
+      (* TODO simplify these using context as a function *)
+      (* apply mappings to concrete lists *)
+      | |- context [map ?f (cons ?x ?xs) ] => idtac f;
+          let v := eval cbv [map] in (map f (cons x xs)) in change (map f (cons x xs)) with v
+      (* unfold array applications to concrete lists *)
+      | |- context [array ?e ?sz ?p (cons ?x ?xs) ] => 
+          let v := eval cbv [array] in (array e sz p (cons x xs)) in change (array e sz p (cons x xs)) with v
+      (* apply skipn of constants to concrete lists *)
+      | |- context [skipn ?n (cons ?x ?xs)] => lazymatch isNatCst n with true =>
+          let v := eval cbv [skipn] in (skipn n (cons x xs)) in change (skipn n (cons x xs)) with v
+        end
+    end.
+
+    simplify_lists_in_goal.
+
+    (* TODO is this already in the ecancel database? If not, should it be? *)
+    Ltac ptsto_to_sepclause_in p H :=
+      let AR := fresh in
+      epose (array1_iff_eq_of_list_word_at p) as AR; seprewrite_in AR H; [solve_nums|]; clear AR.
+  
+    ptsto_to_sepclause_in a2 H30.
+
+    use_sep_assumption_impl. 
+    
+    cancel.
+    cancel_seps_at_indices_by_implication 0%nat 3%nat. { exact impl1_refl. }
+    cancel_seps_at_indices_by_implication 0%nat 2%nat. {
+      intros ? ?. replace (scalarmult 1 a0) with a0. 2: { admit. (* this needs weakened assumptions *) }
+      exists a_repr. assumption.
+    }
+    cancel_seps_at_indices_by_implication 0%nat 1%nat. {
+      intros ? ?. replace (m1_prep (scalarmult 1 a0)) with (m1_prep a0). 2: { admit. } 
+      exists x1. assumption.
+    }
+    cancel_seps_at_indices_by_implication 0%nat 0%nat. {
+      intros ? ?. replace (m1_prep (scalarmult 0 a0)) with (m1_prep zero). 2: { admit. }
+      exists x0. assumption.
+    }
+    exact impl1_refl.
+
+    ZnWords.
+  }
+  {
+    repeat straightline.
+    {
+      (* Single out i/2 * A from uncached multiples. *)
+      erewrite <- (firstn_skipn_middle (Z.to_nat (word.unsigned x5 /2 - 1)) (skipn 1 (multiples (Z.to_nat (word.unsigned x5)) a0))) in H36. 2: {
+        unshelve erewrite nth_error_nth'. exact a0.
+        2 : { solve_nums. }
+        simplify_lists_in_goal.
+        (* TODO tactic? *)
+        replace (1 + Z.to_nat (word.unsigned x5 / 2 - 1))%nat with (Z.to_nat (word.unsigned x5 / 2))%nat by ZnWords.
+        exact eq_refl.
+      }
+
+      rewrite array_app in H36. seprewrite_in (@array_cons) H36.
+
+      (* TODO how to simplify? *)
+      replace (x6.+200 * Z.of_nat (Datatypes.length (firstn (Z.to_nat (word.unsigned x5 / 2 - 1)) (skipn 1 (multiples (Z.to_nat (word.unsigned x5)) a0))))) with
+        (word.add x6 (word.mul (word.sub (word.sru x5 (word.of_Z 1)) (word.of_Z 1)) (word.of_Z 200))) in H36 by solve_nums.
+      cbv [projective_point] in H36. extract_ex1_and_emp_in H36.
+
+      (* Double (i/2)*A -> temp contains i*A.  *)
+      single_step.
+      repeat straightline.
+      
+      (* split out ai[i]*)
+      split_stack_at_n_in (skipn (Z.to_nat (word.unsigned x5 * 160)) out) (x10.+word.unsigned x5 * 160) 160%nat H41. 
+      (* copy temp into ai[i] *)
+      single_step.
+
+      repeat straightline.
+      (* if condition and saving into p_ai_uncached is next. *)
+      unfold1_cmd_goal; cbv beta match delta [cmd_body].
+      repeat straightline.
+      split. (* if cases - this may get weird cause the rest doesn't depend on the if... *)
+
+      { (*  i < 8 -> copy i*A into p_ai_uncached *)
+      intros.
+      Search not Logic.eq word.unsigned.
+      apply word.if_nonzero in H39.
+      Require Import coqutil.Tactics.autoforward.
+      autoforward with typeclass_instances in H39. 
+
+      (* split off the space for p_ai_uncached[i] *)
+      split_stack_at_n_in (skipn (Z.to_nat ((word.unsigned x5 - 1) * 200)) stack1) (x6.+(word.unsigned x5 - 1) * 200) 200%nat H42.
+
+      (* TODO how to simplify? *)
+      replace (x6.+(word.unsigned x5 - 1) * 200) with (word.add x6 (word.mul (word.sub x5 (word.of_Z 1)) (word.of_Z 200))) in H42 by ZnWords.
+
+      single_step.
+      
+      (* if is done. from here on goal 1 and 2 are the same, I'll need to aggregate them, hope that works. *)
+
+      (*calculate (i+1)*A, store in temp *)
+      single_step.
+      (* length of a byte serialized representative is correct. this is needed to free up temp again using p5@ -> $@ 
+        I'd prefer to have this in a lemma in Field.v, but for now I can do it here. *)
+      { clear -H45.
+        destruct_points.
+        cbv [FElem Bignum.Bignum projective_repr_to_list_byte proj1_sig].
+        rewrite !app_length, !ArrayCasts.ws2bs_length. cbv [projective_repr_to_list_byte proj1_sig FElem Bignum.Bignum] in H45.
+        extract_ex1_and_emp_in H45. rewrite H45_emp0, H45_emp1, H45_emp2, H45_emp3, H45_emp4.
+        change felem_size_in_words with 10%nat. Lia.lia.
+      }
+
+      (* Store (i+1)*A in the result array. *)
+      repeat straightline.
+      (* probably need to single out ai[i+1]? *)
+      split_stack_at_n_in (skipn (160 + Z.to_nat (word.unsigned x5 * 160)) out) (x10.+word.unsigned x5 * 160.+160) 160%nat H46.
+      replace (x10.+word.unsigned x5 * 160.+160) with (word.add x10 (word.mul (x5.+1) (word.of_Z 160))) in H46 by ZnWords.
+      single_step.
+      
+      repeat straightline.
+      (* next if, need to decide if i < 7  *)
+      unfold1_cmd_goal; cbv beta match delta [cmd_body].
+      repeat straightline.
+      split.
+      {
+      (* i < 7 -> copy (i+1)*A into p_ai_uncached*)
+      intros.
+      (* same inconvenience again to actually have that i < 7 in a usable format... *)
+      destruct (word.ltu x5 (word.of_Z 7)) eqn:?.
+      2: { exfalso; apply H43. ZnWords. }
+      assert (word.unsigned x5 < 7). rewrite ?word.unsigned_ltu in *. ZnWords.
+
+      (* split off space for p_ai_uncached[i+1]*)
+      split_stack_at_n_in (skipn (200 + Z.to_nat ((word.unsigned x5 - 1) * 200)) stack1) (word.add x6
+  (word.mul (word.of_Z 200) x5)) 200%nat   H47.
+      replace (word.add x6 (word.mul (word.of_Z 200) x5)) with ((word.add x6 (word.mul x5 (word.of_Z 200)))) in H47 by ZnWords.
+
+      single_step.
+
+      repeat straightline. (* this one takes very long, maybe figure out why? *)
+      change i with (x5.+2).
+      (* why isn't straightline procssing the markers? I can follow them manually.. *)
+      do 3 letexists. split; ssplit. 
+      { repeat straightline. }
+      { ZnWords. }
+      { ZnWords. }
+      { ZnWords. }
+      3: { 
+        split. 
+        { ZnWords. }
+        {
+          repeat straightline.
+          ecancel_assumption.
+        }
+      }
+
+    (* memory invariant is true after the loop. *)
+    replace (firstn (Z.to_nat (word.unsigned (x5.+2))) cached_multiples_a) with 
+      ((firstn (Z.to_nat (word.unsigned x5)) cached_multiples_a) ++
+        [m1_prep (scalarmult (Z.to_nat (word.unsigned x5)) a0)] ++
+        [m1_prep (scalarmult (Z.to_nat (word.unsigned x5) + 1)%nat a0)])%list. 2:{
+          replace (Z.to_nat (word.unsigned (x5.+2))) with (Z.to_nat (word.unsigned x5) + 2)%nat by ZnWords.
+          rewrite firstn_add. 2: {
+            cbv [cached_multiples_a multiples_a]. rewrite length_map, length_multiples. ZnWords.
+          }
+          cbv [cached_multiples_a multiples_a].
+          rewrite (firstn_pick_2 _ (m1_prep a0)). 2: {
+            rewrite length_map, length_multiples. ZnWords.
+          }
+          rewrite !map_nth, !multiples_correct; try ZnWords.
+          exact eq_refl. 
+        }
+    replace (firstn (Z.to_nat (word.unsigned (x5.+2)) - 1) uncached_multiples_a) with 
+      ((firstn (Z.to_nat (word.unsigned x5) - 1) uncached_multiples_a) ++ [scalarmult (Z.to_nat (word.unsigned x5)) a0] ++ [scalarmult (Z.to_nat (word.unsigned x5) + 1)%nat a0])%list. 2: {
+        replace (Z.to_nat (word.unsigned (x5.+2)) - 1)%nat with (Z.to_nat (word.unsigned x5) - 1 + 2)%nat by ZnWords.
+        rewrite firstn_add. 2: {
+          cbv [uncached_multiples_a multiples_a]. rewrite !length_firstn, length_skipn, length_multiples. ZnWords.
+        }
+        cbv [uncached_multiples_a multiples_a].
+        rewrite (firstn_pick_2 _ a0). 2: {
+          rewrite length_firstn, length_skipn, length_multiples. ZnWords.
+        } 
+        (* this is going to be different depending on the if branch we've taken, I hope it works.
+            It should, because if the if is false, we're also not adding any points here. *)
+        rewrite !nth_firstn.
+        replace ((Z.to_nat (word.unsigned x5) - 1 <? 8)%nat) with true. 2: {
+          symmetry. rewrite Nat.ltb_lt. ZnWords.
+        }
+        replace (Z.to_nat (word.unsigned x5) - 1 + 1 <? 8)%nat with true. 2: {
+          symmetry. rewrite Nat.ltb_lt. ZnWords.
+        }
+        rewrite !nth_skipn.
+        rewrite !multiples_correct; try ZnWords.
+        replace (1 + (Z.to_nat (word.unsigned x5) - 1))%nat with (Z.to_nat (word.unsigned x5)) by Lia.lia.
+        replace (1 + (Z.to_nat (word.unsigned x5) - 1 + 1))%nat with (Z.to_nat (word.unsigned x5) + 1)%nat by Lia.lia.
+        exact eq_refl.
+      }
+    rewrite !array_app.
+
+    (* solve the goals and see what else needs reformatting. *)
+    use_sep_assumption_impl. cancel.
+    cancel_seps_at_indices_by_implication 0%nat 6%nat. { (* (i+1) * A in uncached_multiples *)
+      cbv [array uncached_multiples_a multiples_a].
+      rewrite !length_firstn, length_skipn, length_multiples.
+      cbv [Datatypes.length]. bottom_up_simpl_in_goal.
+      replace (x6.+200 * Z.of_nat (Init.Nat.min (Z.to_nat (word.unsigned x5) - 1) 8).+200) 
+        with (word.add x6 (word.mul x5 (word.of_Z 200))) by ZnWords.
+      intros ? ?. extract_ex1_and_emp_in_goal.
+      split; [|auto].
+      replace ((scalarmult (Z.to_nat (word.unsigned x5) + 1) a0)) with 
+        (m1add (scalarmult (Z.to_nat (word.unsigned x5)) a0) a0). 2: {
+          replace (Z.to_nat (word.unsigned x5) + 1)%nat with (S (Z.to_nat (word.unsigned x5))) by Lia.lia.
+          unfold scalarmult. fold scalarmult. (* this could be a lemma, makes it easier. *)
+          exact eq_refl.
+      }
+      unshelve eexists.
+      (* wait, actually I need to weaken my statements here. x13 is not going to satisfy this, it's coordinates
+      are not equal to m1add.. projective_repr p needs to be a representative up to point equality. *)
+      
+
+
+
+End WithParameters.
